Semantics/Imp/Denotational.lean
@@ -26,8 +26,8 @@ theorem monotone_denote_loop: monotone (denote_while b c) :=
 
 notation (priority := high) "[[" c "]]" => denote c
 
-#check (s0, s0["x"<-5]["x"<-1]) ∈ [[[|x := 5; if x <= 1 then skip else x := 1 end|]]]
-#check (s0, s0["x"<-5]) ∈ [[[|x := 5; while x <= 1 loop x := 1 end|]]]
+#check (s0, s0["x"<-5]["x"<-1]) ∈ [[[|x = 5; if x <= 1 {skip} else {x = 1}|]]]
+#check (s0, s0["x"<-5]) ∈ [[[|x = 5; while x <= 1 {x = 1}|]]]
 
 namespace Denotational
 
