Semantics/Imp/Lang.lean
@@ -17,11 +17,11 @@ inductive Aexp where
   | sub : Aexp -> Aexp -> Aexp
   | mul : Aexp -> Aexp -> Aexp
 
-instance: OfNat Aexp n := ⟨Aexp.val n⟩
-instance: Add Aexp := ⟨Aexp.add⟩
-instance: Sub Aexp := ⟨Aexp.sub⟩
-instance: Neg Aexp := ⟨(Aexp.sub 0 .)⟩
-instance: Mul Aexp := ⟨Aexp.mul⟩
+instance: OfNat Aexp n := ⟨.val n⟩
+instance: Add Aexp := ⟨.add⟩
+instance: Sub Aexp := ⟨.sub⟩
+instance: Neg Aexp := ⟨(.sub 0 .)⟩
+instance: Mul Aexp := ⟨.mul⟩
 
 -- x + 3
 #check Aexp.var "x" + 3
@@ -41,21 +41,22 @@ inductive Bexp where
   | eq : Aexp -> Aexp -> Bexp
   | le : Aexp -> Aexp -> Bexp
 
-instance: Complement Bexp := ⟨Bexp.not⟩
-instance: AndOp Bexp := ⟨Bexp.and⟩
-instance: OrOp Bexp := ⟨Bexp.or⟩
+instance: Complement Bexp := ⟨.not⟩
+instance: AndOp Bexp := ⟨.and⟩
+instance: OrOp Bexp := ⟨.or⟩
 
 -- !(x <= 3)
 #check ~~~(Bexp.le (Aexp.var "x") 3)
 
 inductive Com where
   | skip
-  | cat        : Com -> Com -> Com
-  | ass        : String -> Aexp -> Com
-  | ifElse     : Bexp -> Com -> Com -> Com
-  | whileLoop  : Bexp -> Com -> Com
+  | cat       : Com -> Com -> Com
+  | ass       : String -> Aexp -> Com
+  | ifElse    : Bexp -> Com -> Com -> Com
+  | whileLoop : Bexp -> Com -> Com
 
-instance: Append Com := Append.mk Com.cat
+instance: EmptyCollection Com := ⟨.skip⟩
+instance: Append Com := ⟨.cat⟩
 
 /-
 ## Syntax
@@ -74,47 +75,47 @@ syntax:60 imp:60 "-" imp:61 : imp
 -- bexp
 syntax:65 imp:65 "&&" imp:66 : imp
 syntax:65 imp:65 "||" imp:66 : imp
-syntax:70 imp:70 "=" imp:71 : imp
+syntax:70 imp:70 "==" imp:71 : imp
 syntax:70 imp:70 "<=" imp:71 : imp
 syntax:80 "!" imp:81 : imp
 -- com
 syntax:40 imp:40 ";" imp:41 : imp
-syntax:50 imp:50 ":=" imp:51 : imp
-syntax "if" imp "then" imp "else" imp "end" : imp
-syntax "while" imp "loop" imp "end" : imp
+syntax:50 imp:50 "=" imp:51 : imp
+syntax "if" imp "{" imp "}" "else" "{" imp "}" : imp
+syntax "while" imp "{" imp "}" : imp
 -- meta
 syntax "[|" imp "|]" : term
 
 macro_rules
-  -- keywords
-  | `([|skip|]) => `(Com.skip)
-  | `([|true|]) => `(Bexp.true)
-  | `([|false|]) => `(Bexp.false)
-  -- general
-  | `([|($x)|]) => `([|$x|])
-  -- aexp
-  | `([|$x:ident|]) => `(Aexp.var $(Lean.quote (toString x.getId)))
-  | `([|$n:num|])   => `($n)
-  | `([|$x + $y|])  => `([|$x|] + [|$y|])
-  | `([|$x - $y|])  => `([|$x|] - [|$y|])
-  | `([|$x * $y|])  => `([|$x|] * [|$y|])
-  -- bexp
-  | `([|!$x|])      => `(~~~[|$x|])
-  | `([|$x && $y|]) => `([|$x|] &&& [|$y|])
-  | `([|$x || $y|]) => `([|$x|] ||| [|$y|])
-  | `([|$x = $y|]) => `(Bexp.eq [|$x|] [|$y|])
-  | `([|$x <= $y|]) => `(Bexp.le [|$x|] [|$y|])
-  -- com
-  | `([|$x:ident := $y|]) => `(Com.ass $(Lean.quote (toString x.getId)) [|$y|])
-  | `([|$x ; $y|])       => `(Com.cat [|$x|] [|$y|])
-  | `([|if $b then $x else $y end|]) => `(Com.ifElse [|$b|] [|$x|] [|$y|])
-  | `([|while $b loop $x end|]) => `(Com.whileLoop [|$b|] [|$x|])
+-- keywords
+| `([|skip|]) => `(Com.skip)
+| `([|true|]) => `(Bexp.true)
+| `([|false|]) => `(Bex.false)
+-- general
+| `([|($x)|]) => `([|$x|])
+-- aexp
+| `([|$x:ident|]) => `(Aexp.var $(Lean.quote x.getId.toString))
+| `([|$n:num|])   => `($n)
+| `([|$x + $y|])  => `([|$x|] + [|$y|])
+| `([|$x - $y|])  => `([|$x|] - [|$y|])
+| `([|$x * $y|])  => `([|$x|] * [|$y|])
+-- bexp
+| `([|!$x|])      => `(~~~[|$x|])
+| `([|$x && $y|]) => `([|$x|] &&& [|$y|])
+| `([|$x || $y|]) => `([|$x|] ||| [|$y|])
+| `([|$x == $y|]) => `(Bexp.eq [|$x|] [|$y|])
+| `([|$x <= $y|]) => `(Bexp.le [|$x|] [|$y|])
+-- com
+| `([|$x:ident = $y|]) => `(Com.ass $(Lean.quote x.getId.toString) [|$y|])
+| `([|$x ; $y|])       => `(Com.cat [|$x|] [|$y|])
+| `([|if $b {$x} else {$y}|]) => `(Com.ifElse [|$b|] [|$x|] [|$y|])
+| `([|while $b {$x}|]) => `(Com.whileLoop [|$b|] [|$x|])
 
 #check [|
-n := 5; i := 2; res := 1;
+  n = 5; i = 2; res = 1;
 
-while i <= n loop
-    res := res * i;
-    i := i + 1
-end
+  while i <= n {
+      res = res * i;
+      i = i + 1
+  }
 |]
